tests/lean/run/dunfold2.lean
@@ -1,0 +1,52 @@
+open tactic
+
+set_option pp.all true
+
+def g : nat → nat := λ x, x + 5
+
+example (a b : nat) (p : nat → Prop) (h : p (g (nat.succ (nat.succ a)))) : p (g (a + 2)) :=
+by do
+  t ← target,
+  new_t ← dsimplify (λ e, failed)
+     (λ e,
+        do { new_e ← unfold_projection e, return (new_e, tt) }
+        <|>
+        do {
+         guard ([`add, `nat.add, `one, `zero]^.any e^.is_app_of),
+         /- We are using transparency.none, so
+
+            nat.add a (bit0 (nat.succ nat.zero))
+
+            cannot be matched with
+
+            nat.add ?a (nat.succ ?b)
+         -/
+         new_e ← dunfold_expr_core transparency.none e, trace e,
+         trace "===>", trace new_e, trace "-------",
+         return (new_e, tt) })
+     t,
+  trace new_t,
+  expected ← to_expr `(p (g (nat.add a (bit0 (nat.succ nat.zero))))),
+  guard (new_t = expected),
+  trace new_t,
+  assumption
+
+
+example (a b : nat) (p : nat → Prop) (h : p (g (nat.succ (nat.succ a)))) : p (g (a + nat.succ (nat.succ 0))) :=
+by do
+  t ← target,
+  new_t ← dsimplify (λ e, failed)
+     (λ e,
+        do { new_e ← unfold_projection e, return (new_e, tt) }
+        <|>
+        do {
+         guard ([`add, `nat.add, `one, `zero]^.any e^.is_app_of),
+         new_e ← dunfold_expr_core transparency.none e, trace e,
+         trace "===>", trace new_e, trace "-------",
+         return (new_e, tt) })
+     t,
+  trace new_t,
+  expected ← to_expr `(p (g (nat.succ (nat.succ a)))),
+  guard (new_t = expected),
+  trace new_t,
+  assumption
